theories/LogicalRelation/NormalRed.v
@@ -2,13 +2,13 @@
 From Coq Require Import CRelationClasses.
 From LogRel.AutoSubst Require Import core unscoped Ast Extra.
 From LogRel Require Import Utils BasicAst Notations Context NormalForms UntypedReduction Weakening GenericTyping LogicalRelation.
-From LogRel.LogicalRelation Require Import Induction Irrelevance Escape Reflexivity Weakening Neutral Transitivity Reduction.
+From LogRel.LogicalRelation Require Import Induction Irrelevance Escape Reflexivity Weakening Neutral Transitivity Reduction EqRedRight.
 
 Set Universe Polymorphism.
 
 Ltac redSubst :=
   match goal with
-  | [H : [_ |- ?X :⤳*: ?Y] |- _] => 
+  | [H : [_ |- ?X :⤳*: ?Y] |- _] =>
     assert (X = Y)by (eapply redtywf_whnf ; gen_typing); subst; clear H
   end.
 
@@ -31,18 +31,18 @@ Program Definition normRedΠ0 {Γ F G l} (h : [Γ ||-Π<l> tProd F G])
   : [Γ ||-Π<l> tProd F G] :=
   {| PiRedTyPack.dom := F ;
      PiRedTyPack.cod := G |}.
-Solve All Obligations with 
+Solve All Obligations with
   intros; pose proof (e := redtywf_whnf (PiRedTyPack.red h) whnf_tProd);
-  symmetry in e; injection e; clear e; 
+  symmetry in e; injection e; clear e;
   destruct h ; intros; cbn in *; subst; eassumption.
 
 Program Definition normRedΣ0 {Γ F G l} (h : [Γ ||-Σ<l> tSig F G])
   : [Γ ||-Σ<l> tSig F G] :=
   {| PiRedTyPack.dom := F ;
      PiRedTyPack.cod := G |}.
-Solve All Obligations with 
+Solve All Obligations with
   intros; pose proof (e := redtywf_whnf (PiRedTyPack.red h) whnf_tSig);
-  symmetry in e; injection e; clear e; 
+  symmetry in e; injection e; clear e;
   destruct h ; intros; cbn in *; subst; eassumption.
 
 Definition normRedΠ {Γ F G l} (h : [Γ ||-<l> tProd F G]) : [Γ ||-<l> tProd F G] :=
@@ -52,7 +52,7 @@ Definition normRedΣ {Γ F G l} (h : [Γ ||-<l> tSig F G]) : [Γ ||-<l> tSig F G
   LRSig' (normRedΣ0 (invLRΣ h)).
 
 #[program]
-Definition normEqRedΣ {Γ F F' G G' l} (h : [Γ ||-<l> tSig F G]) 
+Definition normEqRedΣ {Γ F F' G G' l} (h : [Γ ||-<l> tSig F G])
   (heq : [Γ ||-<l> _ ≅ tSig F' G' | h]) : [Γ ||-<l> _ ≅ tSig F' G' | normRedΣ h] :=
   {|
     PiRedTyEq.dom := F';
@@ -61,29 +61,49 @@ Definition normEqRedΣ {Γ F F' G G' l} (h : [Γ ||-<l> tSig F G])
 Solve All Obligations with
   intros; assert[Γ ||-<l> _ ≅ tSig F' G' | normRedΣ h] as [?? red] by irrelevance;
   pose proof (e := redtywf_whnf red whnf_tSig);
-  symmetry in e; injection e; clear e; 
+  symmetry in e; injection e; clear e;
   destruct h ; intros; cbn in *; subst; eassumption.
 
 #[program]
-Definition normLambda {Γ F F' G t l RΠ} 
-  (Rlam : [Γ ||-<l> tLambda F' t : tProd F G | normRedΠ RΠ ]) :
-  [Γ ||-<l> tLambda F' t : tProd F G | normRedΠ RΠ ] :=
-  {| PiRedTm.nf := tLambda F' t |}.
+Definition normRedId0 {Γ A x y l} (h : [Γ ||-Id<l> tId A x y])
+  : [Γ ||-Id<l> tId A x y] :=
+  mkIdRedTy A x y _ _ _ _.
 Solve All Obligations with
-  intros;
-  pose proof (e := redtmwf_whnf (PiRedTm.red Rlam) whnf_tLambda);
-  destruct Rlam as [???? app eqq]; cbn in *; subst;
-  first [eapply app | now eapply eqq| eassumption].
+  intros; pose proof (e := redtywf_whnf (IdRedTy.red h) whnf_tId);
+  symmetry in e; injection e; clear e;
+  destruct h ; intros; cbn in *; subst;
+  first [eassumption | irrelevance].
+
+Definition normRedId {Γ A x y l} (h : [Γ ||-<l> tId A x y]) : [Γ ||-<l> tId A x y] :=
+  LRId' (normRedId0 (invLRId h)).
 
 #[program]
-Definition normPair {Γ F F' G G' f g l RΣ} 
-  (Rp : [Γ ||-<l> tPair F' G' f g : tSig F G | normRedΣ RΣ ]) :
-  [Γ ||-<l> tPair F' G' f g : tSig F G | normRedΣ RΣ ] :=
-  {| SigRedTm.nf := tPair F' G' f g |}.
+Definition normLambda {Γ F Fl Fr G tl tr l RΠ}
+  (Rlam : [Γ ||-<l> tLambda Fl tl ≅ tLambda Fr tr : tProd F G | normRedΠ RΠ ]) :
+  [Γ ||-<l> tLambda Fl tl ≅ tLambda Fr tr : tProd F G | normRedΠ RΠ ] :=
+  {|
+    PiRedTmEq.redL := {| PiRedTmEq.nf := tLambda Fl tl |} ;
+    PiRedTmEq.redR := {| PiRedTmEq.nf := tLambda Fr tr |}
+  |}.
 Solve All Obligations with
   intros;
-  pose proof (e := redtmwf_whnf (SigRedTm.red Rp) whnf_tPair);
-  destruct Rp as [???? fstRed sndRed]; cbn in *; subst;
+  pose proof (eL := redtmwf_whnf (PiRedTmEq.red Rlam.(PiRedTmEq.redL)) whnf_tLambda);
+  pose proof (eR := redtmwf_whnf (PiRedTmEq.red Rlam.(PiRedTmEq.redR)) whnf_tLambda);
+  destruct Rlam as [[] [] app eqq]; cbn in *; subst;
+  first [eapply app | now eapply eqq| eassumption].
+
+
+#[program]
+Definition normPair {Γ F Fl Fr G Gl Gr fl fr gl gr l RΣ}
+  (Rp : [Γ ||-<l> tPair Fl Gl fl gl ≅ tPair Fr Gr fr gr : tSig F G | normRedΣ RΣ ]) :
+  [Γ ||-<l> tPair Fl Gl fl gl ≅ tPair Fr Gr fr gr : tSig F G | normRedΣ RΣ ] :=
+  {| SigRedTmEq.redL := {| SigRedTmEq.nf := tPair Fl Gl fl gl |} ;
+     SigRedTmEq.redR := {| SigRedTmEq.nf := tPair Fr Gr fr gr |} |}.
+Solve All Obligations with
+  intros;
+  pose proof (eL := redtmwf_whnf (SigRedTmEq.red (SigRedTmEq.redL Rp)) whnf_tPair);
+  pose proof (eR := redtmwf_whnf (SigRedTmEq.red (SigRedTmEq.redR Rp)) whnf_tPair);
+  destruct Rp as [[] [] ? fstRed sndRed]; cbn in *; subst;
   first [eapply fstRed | irrelevanceRefl; now unshelve eapply sndRed| eassumption].
 
 Definition invLRcan {Γ l A} (lr : [Γ ||-<l> A]) (w : isType A) : [Γ ||-<l> A] :=
@@ -96,7 +116,6 @@ Definition invLRcan {Γ l A} (lr : [Γ ||-<l> A]) (w : isType A) : [Γ ||-<l> A]
   | IdType => fun _ x => LRId' x
   | NeType wh => fun _ x => LRne_ _ (normRedNe0 x wh)
   end lr (invLR lr (reflexivity A) w).
-  
 
 End Normalization.
 
@@ -107,10 +126,10 @@ End Normalization.
 Ltac normRedΠin X :=
   let g := type of X in
   match g with
-  | [ LRAd.pack ?R | _ ||- ?t : _] =>
+  (* | [ LRAd.pack ?R | _ ||- ?t : _] =>
     let X' := fresh X in
     rename X into X' ;
-    assert (X : [_ ||-<_> t : _ | LRPi' (normRedΠ0 (invLRΠ R))]) by irrelevance; clear X'
+    assert (X : [_ ||-<_> t : _ | LRPi' (normRedΠ0 (invLRΠ R))]) by irrelevance; clear X' *)
   | [ LRAd.pack ?R | _ ||- _ ≅ ?B] =>
     let X' := fresh X in
     rename X into X' ;
@@ -123,12 +142,12 @@ Ltac normRedΠin X :=
 
 Goal forall `{GenericTypingProperties} Γ A B l R f X
   (RABX : [Γ ||-<l> arr A B ≅ X | R])
-  (Rf : [Γ ||-<l> f : arr A B | R])
+  (* (Rf : [Γ ||-<l> f : arr A B | R]) *)
   (Rff : [Γ ||-<l> f ≅ f : arr A B | R])
 , True.
 Proof.
   intros.
-  normRedΠin Rf.
+  (* normRedΠin Rf. *)
   normRedΠin Rff.
   normRedΠin RABX.
   constructor.
@@ -151,10 +170,10 @@ Ltac normRedΠ id :=
 Ltac normRedΣin X :=
   let g := type of X in
   match g with
-  | [ LRAd.pack ?R | _ ||- ?t : _] =>
+  (* | [ LRAd.pack ?R | _ ||- ?t : _] =>
     let X' := fresh X in
     rename X into X' ;
-    assert (X : [_ ||-<_> t : _ | LRSig' (normRedΣ0 (invLRΣ R))]) by irrelevance; clear X'
+    assert (X : [_ ||-<_> t : _ | LRSig' (normRedΣ0 (invLRΣ R))]) by irrelevance; clear X' *)
   | [ LRAd.pack ?R | _ ||- _ ≅ ?B] =>
     let X' := fresh X in
     rename X into X' ;
