theories/LogicalRelation/Id.v
@@ -1,38 +1,12 @@
 From LogRel.AutoSubst Require Import core unscoped Ast Extra.
 From LogRel Require Import Notations Utils BasicAst Context NormalForms Weakening GenericTyping LogicalRelation.
-From LogRel.LogicalRelation Require Import Induction Irrelevance Weakening Neutral Escape Reflexivity NormalRed Reduction Transitivity Universe.
+From LogRel.LogicalRelation Require Import Induction Escape Irrelevance Weakening Neutral Reflexivity NormalRed Reduction Transitivity Universe EqRedRight.
 
 Set Universe Polymorphism.
 Set Printing Primitive Projection Parameters.
 
 Section IdRed.
   Context `{GenericTypingProperties}.
-
-  Lemma mkIdRedTy {Γ l A} :
-    forall (ty lhs rhs  : term)
-      (tyRed : [Γ ||-<l> ty]),
-      [Γ |- A :⤳*: tId ty lhs rhs] ->
-      [tyRed | Γ ||- lhs : _] ->
-      [tyRed | Γ ||- rhs : _] ->
-      [Γ ||-Id<l> A].
-  Proof.
-    intros; unshelve econstructor; cycle 3; tea.
-    1: intros; now eapply wk.
-    2,3: now eapply reflLRTmEq.
-    2: apply perLRTmEq.
-    - eapply  convty_Id. 
-      1: eapply escapeEq; now eapply reflLRTyEq.
-      1,2: eapply escapeEqTerm; now eapply reflLRTmEq.
-    - cbn; intros; irrelevance0; [|now eapply wkEq].
-      bsimpl; rewrite H11; now bsimpl.
-      Unshelve. all:tea.
-    - cbn; intros; irrelevance0; [| now eapply wkTerm].
-      bsimpl; rewrite H11; now bsimpl.
-      Unshelve. all:tea.
-    - cbn; intros; irrelevance0; [| now eapply wkTermEq].
-      bsimpl; rewrite H11; now bsimpl.
-      Unshelve. all:tea.
-  Defined.
 
   Lemma IdRed0 {Γ l A t u} (RA : [Γ ||-<l> A]) :
       [RA | Γ ||- t : _] ->
@@ -43,20 +17,20 @@ Section IdRed.
     1: eapply redtywf_refl; escape; gen_typing.
     all: tea.
   Defined.
-  
+
   Lemma IdRed {Γ l A t u} (RA : [Γ ||-<l> A]) :
       [RA | Γ ||- t : _] ->
       [RA | Γ ||- u : _] ->
       [Γ ||-<l> tId A t u].
   Proof. intros; apply LRId'; now eapply IdRed0. Defined.
-  
+
   Lemma IdRedTy_inv {Γ l A t u} (RIA : [Γ ||-Id<l> tId A t u]) :
     [× A = RIA.(IdRedTy.ty), t = RIA.(IdRedTy.lhs) & u = RIA.(IdRedTy.rhs)].
   Proof.
     pose proof (redtywf_whnf RIA.(IdRedTy.red) whnf_tId) as e; injection e; now split.
   Qed.
 
-  Lemma IdCongRed {Γ l A A' t t' u u'} 
+  Lemma IdCongRed {Γ l A A' t t' u u'}
     (RA : [Γ ||-<l> A])
     (RIA : [Γ ||-<l> tId A t u]) :
     [Γ |- tId A' t' u'] ->
@@ -74,70 +48,60 @@ Section IdRed.
     + irrelevance.
     + cbn; rewrite <- elhs; irrelevance.
     + cbn; rewrite <- erhs; irrelevance.
-  Qed. 
-    
-  Lemma IdRedU@{i j k l} {Γ l A t u}
+  Qed.
+
+  (* Lemma IdRedU@{i j k l} {Γ l A t u}
       (RU : [LogRel@{i j k l} l | Γ ||- U])
       (RU' := invLRU RU)
       (RA : [LogRel@{i j k l} (URedTy.level RU') | Γ ||- A]) :
-      [RU | Γ ||- A : U] ->
-      [RA | Γ ||- t : _] ->
-      [RA | Γ ||- u : _] ->
+      [RU | Γ ||- A ≅ A' : U] ->
+      [RA | Γ ||- t ≅ t': _] ->
+      [RA | Γ ||- u ≅: _] ->
       [RU | Γ ||- tId A t u : U].
   Proof.
     intros RAU Rt Ru.
     enough [LRU_ RU' | _ ||- tId A t u : U] by irrelevance.
     econstructor.
-    - eapply redtmwf_refl; escape; now eapply ty_Id.
+    (* - eapply redtmwf_refl; escape; now eapply ty_Id. *)
     - constructor.
     - eapply convtm_Id; eapply escapeEq + eapply escapeEqTerm; now eapply reflLRTmEq + eapply reflLRTyEq.
     - eapply RedTyRecBwd. eapply IdRed; irrelevanceCum.
     Unshelve. irrelevanceCum.
-  Qed.
-  
-  Lemma IdCongRedU@{i j k l} {Γ l A A' t t' u u'} 
+  Qed. *)
+
+  Lemma IdCongRedU@{i j k l} {Γ l A A' t t' u u'}
       (RU : [LogRel@{i j k l} l | Γ ||- U])
       (RU' := invLRU RU)
-      (RA : [LogRel@{i j k l} (URedTy.level RU') | Γ ||- A])
-      (RA' : [LogRel@{i j k l} (URedTy.level RU') | Γ ||- A']) :
+      (RA : [LogRel@{i j k l} (URedTy.level RU') | Γ ||- A]) :
     [RU | Γ ||- A : U] ->
-    [RU | Γ ||- A' : U] ->
     [RU | _ ||- A ≅ A' : U] ->
-    [RA | _ ||- t : _] ->
-    [RA' | _ ||- t' : _] ->
     [RA | _ ||- t ≅ t' : _] ->
-    [RA | _ ||- u : _] ->
-    [RA' | _ ||- u' : _] ->
     [RA | _ ||- u ≅ u' : _] ->
     [RU | _ ||- tId A t u ≅ tId A' t' u' : U].
   Proof.
-    intros RAU RAU' RAAU' Rt Rt' Rtt' Ru Ru' Ruu'.
+    intros RAU RAAU' Rtt' Ruu'.
     enough [LRU_ RU' | _ ||- tId A t u ≅ tId A' t' u': U] by irrelevance.
-    opector.
-    - change [LRU_ RU' | _ ||- tId A t u : _].
-      enough [RU | _ ||- tId A t u : _] by irrelevance. 
-      now unshelve eapply IdRedU.
-    - change [LRU_ RU' | _ ||- tId A' t' u' : _]. 
-      enough [RU | _ ||- tId A' t' u' : _] by irrelevance. 
-      now unshelve eapply IdRedU.
-    - eapply RedTyRecBwd. eapply IdRed; irrelevanceCum.
-      Unshelve. clear dependent RA'; irrelevanceCum.
+    assert (hAA' : [RA | _ ||- A ≅ A']).
+    1: unshelve eapply UnivEqEq; try irrelevance + irrelevanceCum0.
+    escape. opector.
+    1,2: eexists (tId _ _ _); [eapply redtmwf_refl; gen_typing| constructor].
+    - eapply RedTyRecBwd; unshelve eapply IdRed.
+      all: try eapply lrefl; irrelevanceCum.
     - pose proof (redtmwf_whnf (URedTm.red u0) whnf_tId) as <-.
       pose proof (redtmwf_whnf (URedTm.red u1) whnf_tId) as <-.
-      eapply convtm_Id; now escape.
-    - eapply RedTyRecBwd. eapply IdRed; irrelevanceCum.
-      Unshelve. irrelevanceCum.
+      now eapply convtm_Id.
+    - eapply RedTyRecBwd; unshelve eapply IdRed.
+      1: unshelve eapply UnivEq; [| |irrelevanceCum0| symmetry; irrelevanceCum].
+      all: eapply urefl; eapply LRTmEqConv; tea.
     - eapply TyEqRecFwd.
-      eapply LRTyEqIrrelevantCum.
-      unshelve eapply IdCongRed; tea.
-      + escape; gen_typing.
-      + now eapply UnivEqEq.
-      Unshelve. now eapply IdRed.
+      unshelve eapply LRTyEqIrrelevantCum.
+      2: eapply RedTyRecFwd in l0 ; irrelevanceCum.
+      unshelve eapply IdCongRed; tea; gen_typing.
   Qed.
 
 
 
-Lemma reflRed {Γ l A x} (RA : [Γ ||-<l> A]) (Rx : [RA | _ ||- x : _]) (RIA : [Γ ||-<l> tId A x x]) :
+(* Lemma reflRed {Γ l A x} (RA : [Γ ||-<l> A]) (Rx : [RA | _ ||- x : _]) (RIA : [Γ ||-<l> tId A x x]) :
   [RIA | _ ||- tRefl A x : _].
 Proof.
   set (RIA' := invLRId RIA).
@@ -157,374 +121,162 @@ Proof.
   Unshelve.  all: tea.
 Qed.
 
-Lemma reflRed' {Γ l A x} (RA : [Γ ||-<l> A]) (Rx : [RA | _ ||- x : _]) 
+Lemma reflRed' {Γ l A x} (RA : [Γ ||-<l> A]) (Rx : [RA | _ ||- x : _])
   (RIA := IdRed RA Rx Rx): [RIA | _ ||- tRefl A x : _].
-Proof. now eapply reflRed. Qed.
+Proof. now eapply reflRed. Qed. *)
 
-
-Lemma reflCongRed {Γ l A A' x x'} 
+Lemma reflCongRed {Γ l A A' x x'}
   (RA : [Γ ||-<l> A])
-  (TA' : [Γ |- A'])
-  (RAA' : [RA | _ ||- _ ≅ A'])
-  (Rx : [RA | _ ||- x : _]) 
-  (Tx' : [Γ |- x' : A'])
-  (Rxx' : [RA | _ ||- x ≅ x' : _]) 
+  (RAA : [RA | _ ||- _ ≅ A'])
+  (Rxx : [RA | _ ||- x ≅ x' : _])
   (RIA : [Γ ||-<l> tId A x x]) :
   [RIA | _ ||- tRefl A x ≅ tRefl A' x' : _].
 Proof.
-  set (RIA' := invLRId RIA).
-  enough [LRId' RIA' | _ ||- tRefl A x ≅ tRefl A' x' : _] by irrelevance.
-  pose proof (IdRedTy_inv RIA') as [eA ex ex'].
-  assert (e : tId (IdRedTy.ty RIA') (IdRedTy.lhs RIA') (IdRedTy.rhs RIA') = tId A x x).
-  1: f_equal; now symmetry.
-  assert [Γ |- tId A x x ≅ tId A' x' x'] by (escape ; gen_typing).
-  econstructor; unfold_id_outTy; cbn; rewrite ?e.
-  1,2: eapply redtmwf_refl.
-  1: escape; gen_typing.
-  - eapply ty_conv; [| now symmetry]; now eapply ty_refl.
-  - eapply convtm_refl; now escape.
-  - constructor; cbn.
-    1-4: now escape.  
-    all: irrelevance0; tea.
-    1: apply reflLRTyEq.
-    1,2: rewrite <- ex; tea; now eapply reflLRTmEq.
-    1,2: rewrite <- ex'; tea; now eapply reflLRTmEq.
-  Unshelve. all: tea.
+  set (RIA' := normRedId RIA).
+  enough [RIA' | _ ||- tRefl A x ≅ tRefl A' x' : _] by irrelevance.
+  escape.
+  assert [Γ |- tId A' x' x' ≅ tId A x x] by (symmetry; timeout 1 gen_typing).
+  (* assert [Γ |- tId Ar xr xr ≅ tId A x x] by (symmetry; timeout 1 gen_typing). *)
+  exists (tRefl A x) (tRefl A' x').
+  1,2: eapply redtmwf_refl; unfold_id_outTy; cbn.
+  1: gen_typing.
+  1: eapply ty_conv; [|tea]; gen_typing.
+  1:  unfold_id_outTy; cbn; timeout 1 gen_typing.
+  constructor; tea.
+  1: eapply ty_conv; tea.
+  all: try irrelevance.
+  2,3: eapply lrefl; cbn; irrelevance.
+  eapply reflLRTyEq.
 Qed.
 
-Definition idElimProp {Γ l} (A x P hr y e : term) {IA : [Γ ||-Id<l> tId A x y]} (Pe : IdProp IA e) : term :=
-  match Pe with
-  | IdRedTm.reflR _ _ _ _ _ => hr
-  | IdRedTm.neR _ => tIdElim A x P hr y e
-  end.
 
-Lemma idElimPropIrr {Γ l} {A x P hr y e : term} {IA : [Γ ||-Id<l> tId A x y]} (Pe Pe' : IdProp IA e) :
-  idElimProp A x P hr y e Pe = idElimProp A x P hr y e Pe'.
-Proof.
-  destruct Pe; cbn.
-  2: dependent inversion Pe'; try reflexivity.
-  2:  subst; match goal with H : [_ ||-NeNf _ : _] |- _ => destruct H as [_ ?%convneu_whne]; inv_whne end; tea.
-  refine (match Pe' as Pe0  in IdRedTm.IdProp _ e return match e as e return IdProp _ e -> Type with | tRefl A0 x0 => fun Pe0 => hr = idElimProp A x P hr y (tRefl A0 x0) Pe0 | _ => fun _ => unit end Pe0 with | IdRedTm.reflR _ _ _ _ _ => _ | IdRedTm.neR r  => _ end).
-  1: reflexivity.
-  1: match type of r with [_ ||-NeNf ?t : _] =>  destruct t ; try easy end. 
-  exfalso; destruct r as [_ ?%convneu_whne]; inv_whne.
-Qed.
-
-Lemma IdProp_refl_inv {Γ l A x y A' x'} {IA : [Γ ||-Id<l> tId A x y]} (Pe : IdProp IA (tRefl A' x')) :
-  IdProp IA (tRefl A' x').
-Proof.
-  econstructor; inversion Pe.
-  all: try match goal with H : [_ ||-NeNf _ : _] |- _ => destruct H as [_ ?%convneu_whne]; inv_whne end; tea.
-Defined.
-
-Lemma IdRedTm_whnf_prop {Γ l A x y e} {IA : [Γ ||-Id<l> tId A x y]} (Re : [_ ||-Id<l> e : _ | IA]) :
-  whnf e -> IdProp IA e.
-Proof.
-  intros wh; rewrite (redtmwf_whnf (IdRedTm.red Re) wh).
-  exact (IdRedTm.prop Re).
-Qed.
-
-Lemma idElimPropRed {Γ l A x P hr y e}
+Lemma reflCongRed' {Γ l A Al Ar x xl xr}
   (RA : [Γ ||-<l> A])
-  (Rx : [RA | _ ||- x : _])
-  (RP0 : [Γ ,, A ,, tId A⟨@wk1 Γ A⟩ x⟨@wk1 Γ A⟩ (tRel 0) ||-<l> P])
-  (RP : forall y e (Ry : [RA | Γ ||- y : _]) (RIAxy : [Γ ||-<l> tId A x y]),
-    [ RIAxy | _ ||- e : _] -> [Γ ||-<l> P[e .: y..]])
-  (RPeq : forall A' x' y y' e e' 
-    (RA' : [Γ ||-<l> A'])
-    (RAA' : [RA | _ ||- _ ≅ A'])
-    (Rx' : [RA | _ ||- x' : _])
-    (Rxx' : [RA | _ ||- x ≅ x' : _])
-    (Ry : [RA | Γ ||- y : _])
-    (Ry' : [RA' | _ ||- y' : _])
-    (Ryy' : [RA | Γ ||- y ≅ y' : _])
-    (RIAxy : [Γ ||-<l> tId A x y])
-    (RIAxy' : [Γ ||-<l> tId A x y'])
-    (Re : [ RIAxy | _ ||- e : _])
-    (Re' : [ RIAxy' | _ ||- e' : _])
-    (Ree' : [ RIAxy | _ ||- e ≅ e' : _]),
-    [RP y e Ry RIAxy Re | Γ ||- P[e .: y..] ≅ P[e' .: y' ..]])
-  (Rhr : [RP x (tRefl A x) Rx (IdRed RA Rx Rx) (reflRed' RA Rx) | _ ||- hr : _])
-  (Ry : [RA | _ ||- y : _])
-  (RIAxy : [Γ ||-<l> tId A x y])
-  (Re : [RIAxy | _ ||- e : _]) 
-  (RIAxy0 : [Γ ||-Id<l> tId A x y])
-  (Pe : IdProp RIAxy0 e) :
-  [RP y e Ry _ Re | _ ||- tIdElim A x P hr y e : _] ×
-  [RP y e Ry _ Re | _ ||- tIdElim A x P hr y e ≅ idElimProp A x P hr y e Pe : _].
-Proof.
-  pose proof (IdRedTy_inv RIAxy0) as [eA ex ey].
-  eapply redSubstTerm.
-  - destruct Pe; cbn in *.
-    + eapply LRTmRedConv; tea.
-      unshelve eapply RPeq; cycle 3; tea.
-      2,3: eapply transEqTerm; [|eapply LRTmEqSym]; rewrite ?ex, ?ey; irrelevance.
-      * eapply reflLRTyEq.
-      * eapply reflCongRed; tea.
-        1: irrelevance0; [symmetry; tea|]; tea.
-        rewrite ex; irrelevance.
-    + eapply neuTerm.
-      * escape; eapply ty_IdElim; tea.
-      * destruct r.
-        pose proof (reflLRTyEq RA).
-        pose proof (reflLRTyEq RP0).
-        pose proof Rx as ?%reflLRTmEq.
-        pose proof Ry as ?%reflLRTmEq.
-        pose proof Rhr as ?%reflLRTmEq.
-        escape; eapply convneu_IdElim; tea.
-        eapply convneu_conv; tea. unfold_id_outTy.
-        rewrite <- eA, <- ex, <- ey; eapply convty_Id; tea.
-  - destruct Pe; cbn in *.
-    + escape; eapply redtm_idElimRefl; tea.
-      * eapply ty_conv; tea; rewrite eA; now symmetry.
-      * now rewrite eA.
-      * rewrite eA, ex, ey; etransitivity; tea; now symmetry.
-      * now rewrite eA, ex.
-    + eapply redtm_refl; escape; now eapply ty_IdElim.
-Qed.
-
-
-Lemma idElimRed {Γ l A x P hr y e}
-  (RA : [Γ ||-<l> A])
-  (Rx : [RA | _ ||- x : _])
-  (RP0 : [Γ ,, A ,, tId A⟨@wk1 Γ A⟩ x⟨@wk1 Γ A⟩ (tRel 0) ||-<l> P])
-  (RP : forall y e (Ry : [RA | Γ ||- y : _]) (RIAxy : [Γ ||-<l> tId A x y]),
-    [ RIAxy | _ ||- e : _] -> [Γ ||-<l> P[e .: y..]])
-  (RPeq : forall A' x' y y' e e' 
-    (RA' : [Γ ||-<l> A'])
-    (RAA' : [RA | _ ||- _ ≅ A'])
-    (Rx' : [RA | _ ||- x' : _])
-    (Rxx' : [RA | _ ||- x ≅ x' : _])
-    (Ry : [RA | Γ ||- y : _])
-    (Ry' : [RA' | _ ||- y' : _])
-    (Ryy' : [RA | Γ ||- y ≅ y' : _])
-    (RIAxy : [Γ ||-<l> tId A x y])
-    (RIAxy' : [Γ ||-<l> tId A x y'])
-    (Re : [ RIAxy | _ ||- e : _])
-    (Re' : [ RIAxy' | _ ||- e' : _])
-    (Ree' : [ RIAxy | _ ||- e ≅ e' : _]),
-    [RP y e Ry RIAxy Re | Γ ||- P[e .: y..] ≅ P[e' .: y' ..]])
-  (Rhr : [RP x (tRefl A x) Rx (IdRed RA Rx Rx) (reflRed' RA Rx) | _ ||- hr : _])
-  (Ry : [RA | _ ||- y : _])
-  (RIAxy : [Γ ||-<l> tId A x y])
-  (RIAxy' := LRId' (invLRId RIAxy))
-  (Re : [RIAxy' | _ ||- e : _]) :
-  [RP y e Ry _ Re | _ ||- tIdElim A x P hr y e : _] ×
-  [RP y e Ry _ Re | _ ||- tIdElim A x P hr y e ≅ tIdElim A x P hr y (IdRedTm.nf Re) : _].
-Proof.
-  pose proof (IdRedTy_inv (invLRId RIAxy)) as [eA ex ey].
-  pose proof (hred := Re.(IdRedTm.red)); unfold_id_outTy; rewrite <-eA,<-ex,<-ey in hred.
-  eapply redSubstTerm.
-  - pose proof (redTmFwdConv Re hred (IdProp_whnf _ _ (IdRedTm.prop Re))) as [Rnf Rnfeq].
-    eapply LRTmRedConv.
-    2: eapply idElimPropRed; tea; exact (IdRedTm.prop Re).
-    unshelve eapply LRTyEqSym.
-    2: now eapply RP.
-    eapply RPeq; cycle 2; first [eapply reflLRTyEq | now eapply reflLRTmEq | tea].
-    Unshelve. all: tea.
-  - escape; eapply redtm_idElim; tea; apply hred.
-Qed.
+  (RAAl : [RA | _ ||- _ ≅ Al])
+  (RAAr : [RA | _ ||- _ ≅ Ar])
+  (Rxxl : [RA | _ ||- x ≅ xl : _])
+  (Rxxr : [RA | _ ||- x ≅ xr : _])
+  (RIA : [Γ ||-<l> tId A x x]) :
+  [RIA | _ ||- tRefl Al xl ≅ tRefl Ar xr : _].
+Proof. etransitivity; [symmetry|]; now eapply reflCongRed. Qed.
 
 
 Lemma idElimPropCongRed {Γ l A A' x x' P P' hr hr' y y' e e'}
   (RA : [Γ ||-<l> A])
   (RA' : [Γ ||-<l> A'])
   (RAA' : [RA | Γ ||- A ≅ A'])
-  (Rx : [RA | _ ||- x : _])
-  (Rx' : [RA' | _ ||- x' : _])
   (Rxx' : [RA | _ ||- x ≅ x' : _])
-  (RP0 : [Γ ,, A ,, tId A⟨@wk1 Γ A⟩ x⟨@wk1 Γ A⟩ (tRel 0) ||-<l> P])
-  (RP0' : [Γ ,, A' ,, tId A'⟨@wk1 Γ A'⟩ x'⟨@wk1 Γ A'⟩ (tRel 0) ||-<l> P'])
-  (RPP0 : [RP0 | _ ||- _ ≅ P'])
-  (RP : forall y e (Ry : [RA | Γ ||- y : _]) (RIAxy : [Γ ||-<l> tId A x y]),
-    [ RIAxy | _ ||- e : _] -> [Γ ||-<l> P[e .: y..]])
-  (RP' : forall y' e' (Ry' : [RA' | Γ ||- y' : _]) (RIAxy' : [Γ ||-<l> tId A' x' y']),
-    [ RIAxy' | _ ||- e' : _] -> [Γ ||-<l> P'[e' .: y'..]])
-  (RPP' : forall y y' e e' 
-    (Ry : [RA | Γ ||- y : _])
-    (Ry' : [RA' | Γ ||- y' : _])
+  (RIAxx : [Γ ||-<l> tId A x x])
+  (RP0 : [Γ ,, A ,, tId A⟨@wk1 Γ A⟩ x⟨@wk1 Γ A⟩ (tRel 0) |- P])
+  (RP0' : [Γ ,, A' ,, tId A'⟨@wk1 Γ A'⟩ x'⟨@wk1 Γ A'⟩ (tRel 0) |- P'])
+  (RPP0 : [Γ ,, A ,, tId A⟨@wk1 Γ A⟩ x⟨@wk1 Γ A⟩ (tRel 0) |- P ≅ P'])
+  (RP : forall {y y' e e'} (Ryy' : [RA | Γ ||- y ≅ y' : _]) {RIAxy : [Γ ||-<l> tId A x y]},
+    [ RIAxy | _ ||- e ≅ e' : _] -> [Γ ||-<l> P[e .: y..]])
+  (RPP' : forall y y' e e'
     (Ryy' : [RA | _ ||- y ≅ y' : _])
     (RIAxy : [Γ ||-<l> tId A x y])
-    (RIAxy' : [Γ ||-<l> tId A' x' y'])
-    (Re : [ RIAxy | _ ||- e : _])
-    (Re' : [ RIAxy' | _ ||- e' : _])
     (Ree' : [ RIAxy | _ ||- e ≅ e' : _]),
-    [RP y e Ry _ Re | _ ||- P[e .: y..] ≅ P'[e' .: y'..]])
-  (RPeq : forall A' x' y y' e e' 
-    (RA' : [Γ ||-<l> A'])
+    [RP Ryy' Ree' | _ ||- P[e .: y..] ≅ P'[e' .: y'..]])
+  (RPeq : forall A' x' y y' e e'
     (RAA' : [RA | _ ||- _ ≅ A'])
-    (Rx' : [RA | _ ||- x' : _])
     (Rxx' : [RA | _ ||- x ≅ x' : _])
-    (Ry : [RA | Γ ||- y : _])
-    (Ry' : [RA' | _ ||- y' : _])
     (Ryy' : [RA | Γ ||- y ≅ y' : _])
     (RIAxy : [Γ ||-<l> tId A x y])
-    (RIAxy' : [Γ ||-<l> tId A x y'])
-    (Re : [ RIAxy | _ ||- e : _])
-    (Re' : [ RIAxy' | _ ||- e' : _])
     (Ree' : [ RIAxy | _ ||- e ≅ e' : _]),
-    [RP y e Ry RIAxy Re | Γ ||- P[e .: y..] ≅ P[e' .: y' ..]])
-  (RPeq' : forall A1 x1 y' y1 e' e1 
-    (RA1 : [Γ ||-<l> A1])
-    (RAA1 : [RA' | _ ||- _ ≅ A1])
-    (Rx1 : [RA' | _ ||- x1 : _])
-    (Rxx1 : [RA' | _ ||- x' ≅ x1 : _])
-    (Ry' : [RA' | Γ ||- y' : _])
-    (Ry1 : [RA1 | _ ||- y1 : _])
-    (Ryy1 : [RA' | Γ ||- y' ≅ y1 : _])
-    (RIAxy' : [Γ ||-<l> tId A' x' y'])
-    (RIAxy1 : [Γ ||-<l> tId A' x' y1])
-    (Re' : [ RIAxy' | _ ||- e' : _])
-    (Re1 : [ RIAxy1 | _ ||- e1 : _])
-    (Ree1 : [ RIAxy' | _ ||- e' ≅ e1 : _]),
-    [RP' y' e' Ry' RIAxy' Re' | Γ ||- P'[e' .: y'..] ≅ P'[e1 .: y1 ..]])
-  (Rhr : [RP x (tRefl A x) Rx (IdRed RA Rx Rx) (reflRed' RA Rx) | _ ||- hr : _])
-  (Rhr' : [RP' x' (tRefl A' x') Rx' (IdRed RA' Rx' Rx') (reflRed' RA' Rx') | _ ||- hr' : _])
-  (Rhrhr' : [RP x (tRefl A x) Rx (IdRed RA Rx Rx) (reflRed' RA Rx) | _ ||- hr ≅ hr' : _])
-  (Ry : [RA | _ ||- y : _])
-  (Ry' : [RA' | _ ||- y' : _])
+    [RP Ryy' Ree' | Γ ||- P[e .: y..] ≅ P[e' .: y' ..]])
+  (Rhrhr' : [RP Rxx' (reflCongRed RA RAA' Rxx' RIAxx) | _ ||- hr ≅ hr' : _])
   (Ryy' : [RA | _ ||- y ≅ y' : _])
   (RIAxy : [Γ ||-<l> tId A x y])
-  (RIAxy' : [Γ ||-<l> tId A' x' y'])
-  (Re : [RIAxy | _ ||- e : _]) 
-  (Re' : [RIAxy' | _ ||- e' : _]) 
   (Ree' : [RIAxy | _ ||- e ≅ e' : _])
-  (RIAxy0 : [Γ ||-Id<l> tId A x y])
-  (Pee' : IdPropEq RIAxy0 e e') :
-  [RP y e Ry _ Re | _ ||- tIdElim A x P hr y e ≅ tIdElim A' x' P' hr' y' e' : _].
+  (Pee' : IdPropEq (normRedId0 (invLRId RIAxy)) e e') :
+  [RP Ryy' Ree' | _ ||- tIdElim A x P hr y e ≅ tIdElim A' x' P' hr' y' e' : _].
 Proof.
-  pose proof (IdRedTy_inv RIAxy0) as [eA ex ey].
-  (* pose proof (IdRedTy_inv (invLRId RIAxy))) as [eA ex ey].
-  pose proof (IdRedTy_inv (invLRId RIAxy')) as [eA' ex' ey']. *)
-  pose proof (IdPropEq_whnf _ _ _ Pee') as [whe whe'].
-  assert (Rei : [LRId' RIAxy0 | _ ||- e : _]) by irrelevance.
-  assert (Rei' : [LRId' (invLRId RIAxy') | _ ||- e' : _]) by irrelevance.
-  pose proof (IdRedTm_whnf_prop Rei whe).
-  pose proof (IdRedTm_whnf_prop Rei' whe').
-  eapply LREqTermHelper.
-  1,2: unshelve eapply idElimPropRed; tea.
-  1: now eapply RPP'.
-  destruct Pee'; cbn in *.
-  + unshelve erewrite (idElimPropIrr X), (idElimPropIrr X0).
-    1,2: now eapply IdProp_refl_inv.
-    cbn; eapply LRTmEqRedConv; tea.
-    eapply RPeq; cycle 3; tea.
-    1,4: rewrite ex, ey; eapply transEqTerm; [|eapply LRTmEqSym]; irrelevance.
-    2: eapply reflLRTyEq.
-    eapply reflCongRed; tea.
-    1: irrelevance.
-    rewrite ex; irrelevance.
-  + unshelve erewrite (idElimPropIrr X), (idElimPropIrr X0); destruct r; unfold_id_outTy.
-    * econstructor; escape ; constructor; unfold_id_outTy.
-      1: rewrite <- ex, <- ey, <-eA; tea.
-      now eapply lrefl.
-    * econstructor; pose proof (IdRedTy_inv (invLRId RIAxy')) as [eA' ex' ey'].
-      escape; constructor; unfold_id_outTy.
-      all: rewrite <- ex', <- ey', <-eA'; tea.
-      eapply convneu_conv; [now eapply urefl|].
-      rewrite <- ex, <- ey, <-eA; now eapply convty_Id.
-    * cbn. escape; eapply neuTermEq.
-      - now eapply ty_IdElim.
-      - eapply ty_conv; [now eapply ty_IdElim|].
-        symmetry; eapply escapeEq; now eapply RPP'.
-        Unshelve. all: tea.
-      - eapply convneu_IdElim; tea.
-        now rewrite ex, ey, eA.
+  pose proof (RPP' _ _ _ _ Rxx' _ (reflCongRed RA RAA' Rxx' RIAxx)).
+  pose proof (RPP' _ _ _ _ Ryy' _ Ree').
+  destruct Pee'; cbn in *; escape.
+  - eapply redSubstTmEq; cycle 1.
+    + eapply redtm_idElimRefl; tea.
+      transitivity x'0; [|symmetry]; tea.
+    + eapply redtm_idElimRefl; tea.
+      1-4: eapply ty_conv; tea.
+      1: transitivity A; tea; now symmetry.
+      2: eapply convtm_conv; tea; transitivity x; tea; now symmetry.
+      eapply convtm_conv; tea.
+      transitivity y; tea.
+      transitivity x0; symmetry; tea.
+      transitivity x; tea. now symmetry.
+    + unshelve eapply escapeEq, RPP'; tea.
+    + eapply LRTmEqConv; tea.
+      irrelevanceRefl.
+      eapply RPeq; tea.
+      Unshelve.
+      * transitivity x0; [|symmetry]; irrelevance.
+      * tea.
+      * now eapply reflCongRed.
+  - eapply neuTermEq.
+    + now eapply ty_IdElim.
+    + eapply ty_conv; [|symmetry; tea].
+      eapply ty_IdElim; tea.
+      all: eapply ty_conv; tea.
+      now eapply convty_Id.
+    + eapply convneu_IdElim; tea.
+      destruct r; unfold_id_outTy; now cbn in *.
 Qed.
+
+
+
+
 
 Lemma idElimCongRed {Γ l A A' x x' P P' hr hr' y y' e e'}
   (RA : [Γ ||-<l> A])
   (RA' : [Γ ||-<l> A'])
   (RAA' : [RA | Γ ||- A ≅ A'])
-  (Rx : [RA | _ ||- x : _])
-  (Rx' : [RA' | _ ||- x' : _])
   (Rxx' : [RA | _ ||- x ≅ x' : _])
-  (RP0 : [Γ ,, A ,, tId A⟨@wk1 Γ A⟩ x⟨@wk1 Γ A⟩ (tRel 0) ||-<l> P])
-  (RP0' : [Γ ,, A' ,, tId A'⟨@wk1 Γ A'⟩ x'⟨@wk1 Γ A'⟩ (tRel 0) ||-<l> P'])
-  (RPP0 : [RP0 | _ ||- _ ≅ P'])
-  (RP : forall y e (Ry : [RA | Γ ||- y : _]) (RIAxy : [Γ ||-<l> tId A x y]),
-    [ RIAxy | _ ||- e : _] -> [Γ ||-<l> P[e .: y..]])
-  (RP' : forall y' e' (Ry' : [RA' | Γ ||- y' : _]) (RIAxy' : [Γ ||-<l> tId A' x' y']),
-    [ RIAxy' | _ ||- e' : _] -> [Γ ||-<l> P'[e' .: y'..]])
-  (RPP' : forall y y' e e' 
-    (Ry : [RA | Γ ||- y : _])
-    (Ry' : [RA' | Γ ||- y' : _])
+  (RIAxx : [Γ ||-<l> tId A x x])
+  (RP0 : [Γ ,, A ,, tId A⟨@wk1 Γ A⟩ x⟨@wk1 Γ A⟩ (tRel 0) |- P])
+  (RP0' : [Γ ,, A' ,, tId A'⟨@wk1 Γ A'⟩ x'⟨@wk1 Γ A'⟩ (tRel 0) |- P'])
+  (RPP0 : [Γ ,, A ,, tId A⟨@wk1 Γ A⟩ x⟨@wk1 Γ A⟩ (tRel 0) |- P ≅ P'])
+  (RP : forall {y y' e e'} (Ryy' : [RA | Γ ||- y ≅ y' : _]) {RIAxy : [Γ ||-<l> tId A x y]},
+    [ RIAxy | _ ||- e ≅ e' : _] -> [Γ ||-<l> P[e .: y..]])
+  (RPP' : forall y y' e e'
     (Ryy' : [RA | _ ||- y ≅ y' : _])
     (RIAxy : [Γ ||-<l> tId A x y])
-    (RIAxy' : [Γ ||-<l> tId A' x' y'])
-    (Re : [ RIAxy | _ ||- e : _])
-    (Re' : [ RIAxy' | _ ||- e' : _])
     (Ree' : [ RIAxy | _ ||- e ≅ e' : _]),
-    [RP y e Ry _ Re | _ ||- P[e .: y..] ≅ P'[e' .: y'..]])
-  (RPeq : forall A' x' y y' e e' 
-    (RA' : [Γ ||-<l> A'])
+    [RP Ryy' Ree' | _ ||- P[e .: y..] ≅ P'[e' .: y'..]])
+  (RPeq : forall A' x' y y' e e'
     (RAA' : [RA | _ ||- _ ≅ A'])
-    (Rx' : [RA | _ ||- x' : _])
     (Rxx' : [RA | _ ||- x ≅ x' : _])
-    (Ry : [RA | Γ ||- y : _])
-    (Ry' : [RA' | _ ||- y' : _])
     (Ryy' : [RA | Γ ||- y ≅ y' : _])
     (RIAxy : [Γ ||-<l> tId A x y])
-    (RIAxy' : [Γ ||-<l> tId A x y'])
-    (Re : [ RIAxy | _ ||- e : _])
-    (Re' : [ RIAxy' | _ ||- e' : _])
     (Ree' : [ RIAxy | _ ||- e ≅ e' : _]),
-    [RP y e Ry RIAxy Re | Γ ||- P[e .: y..] ≅ P[e' .: y' ..]])
-  (RPeq' : forall A1 x1 y' y1 e' e1 
-    (RA1 : [Γ ||-<l> A1])
-    (RAA1 : [RA' | _ ||- _ ≅ A1])
-    (Rx1 : [RA' | _ ||- x1 : _])
-    (Rxx1 : [RA' | _ ||- x' ≅ x1 : _])
-    (Ry' : [RA' | Γ ||- y' : _])
-    (Ry1 : [RA1 | _ ||- y1 : _])
-    (Ryy1 : [RA' | Γ ||- y' ≅ y1 : _])
-    (RIAxy' : [Γ ||-<l> tId A' x' y'])
-    (RIAxy1 : [Γ ||-<l> tId A' x' y1])
-    (Re' : [ RIAxy' | _ ||- e' : _])
-    (Re1 : [ RIAxy1 | _ ||- e1 : _])
-    (Ree1 : [ RIAxy' | _ ||- e' ≅ e1 : _]),
-    [RP' y' e' Ry' RIAxy' Re' | Γ ||- P'[e' .: y'..] ≅ P'[e1 .: y1 ..]])
-  (Rhr : [RP x (tRefl A x) Rx (IdRed RA Rx Rx) (reflRed' RA Rx) | _ ||- hr : _])
-  (Rhr' : [RP' x' (tRefl A' x') Rx' (IdRed RA' Rx' Rx') (reflRed' RA' Rx') | _ ||- hr' : _])
-  (Rhrhr' : [RP x (tRefl A x) Rx (IdRed RA Rx Rx) (reflRed' RA Rx) | _ ||- hr ≅ hr' : _])
-  (Ry : [RA | _ ||- y : _])
-  (Ry' : [RA' | _ ||- y' : _])
+    [RP Ryy' Ree' | Γ ||- P[e .: y..] ≅ P[e' .: y' ..]])
+  (Rhrhr' : [RP Rxx' (reflCongRed RA RAA' Rxx' RIAxx) | _ ||- hr ≅ hr' : _])
   (Ryy' : [RA | _ ||- y ≅ y' : _])
   (RIAxy : [Γ ||-<l> tId A x y])
-  (RIAxy' : [Γ ||-<l> tId A' x' y'])
-  (Re : [RIAxy | _ ||- e : _]) 
-  (Re' : [RIAxy' | _ ||- e' : _]) 
-  (Ree' : [RIAxy | _ ||- e ≅ e' : _])  :
-  [RP y e Ry _ Re | _ ||- tIdElim A x P hr y e ≅ tIdElim A' x' P' hr' y' e' : _].
+  (Ree' : [RIAxy | _ ||- e ≅ e' : _]) :
+  [RP Ryy' Ree' | _ ||- tIdElim A x P hr y e ≅ tIdElim A' x' P' hr' y' e' : _].
 Proof.
-  pose proof (IdRedTy_inv (invLRId RIAxy)) as [eA ex ey].
-  assert (RIAxyeq : [RIAxy | _ ||- _ ≅ tId A' x' y']) by (escape; now eapply IdCongRed).
-  assert (Req : [LRId' (invLRId RIAxy) | _ ||- e ≅ e' : _]) by irrelevance.
-  cbn in Req; inversion Req; unfold_id_outTy.
-  pose proof redL as [? _]; pose proof redR as [? _].
-  rewrite <-eA,<-ex,<-ey in redL, redR.
-  pose proof (IdPropEq_whnf _ _ _ prop) as [whL whR].
-  pose proof (redTmFwdConv Re redL whL) as [RnfL RnfLeq].
-  unshelve epose proof (redTmFwdConv Re' _ whR) as [RnfR RnfReq].
-  1: eapply redtmwf_conv; tea; now escape.
-  eapply LREqTermHelper; cycle -1.
-  - eapply LRTmEqRedConv.
-    2: eapply idElimPropCongRed.
-    16: exact prop.
-    all: tea.
-    1: eapply RPeq; cycle 2; first [now eapply reflLRTmEq | now eapply LRTmEqSym| eapply reflLRTyEq| tea].
-    enough [LRId' (invLRId RIAxy) | _ ||- nfL ≅ nfR : _] by irrelevance.
-    exists nfL nfR; tea; eapply redtmwf_refl; unfold_id_outTy; tea.
-  - assert (Re1 : [LRId' (invLRId RIAxy) | _ ||- e : _]) by irrelevance.
-    rewrite (redtmwf_det whL (IdProp_whnf _ _ Re1.(IdRedTm.prop)) redL Re1.(IdRedTm.red)).
-    irrelevanceRefl; eapply idElimRed; tea.
-  - assert (Re1' : [LRId' (invLRId RIAxy') | _ ||- e' : _]) by irrelevance.
-    rewrite (redtmwf_det whR (IdProp_whnf _ _ Re1'.(IdRedTm.prop)) redR Re1'.(IdRedTm.red)).
-    irrelevanceRefl; eapply idElimRed; tea.
-    Unshelve. 
-    all: tea.
-    now eapply RP'.
-  - now eapply RPP'.
+  assert (nRee' : [normRedId RIAxy | Γ ||- e ≅ e' : _]) by irrelevance.
+  destruct nRee' as [nfL nfR ??? prop]; unfold_id_outTy; cbn in *.
+  pose proof (RPP' _ _ _ _ Rxx' _ (reflCongRed RA RAA' Rxx' RIAxx)).
+  pose proof (RPP' _ _ _ _ Ryy' _ Ree').
+  pose proof (IdPropEq_whnf _ _ _ prop) as [].
+  assert (RenfL : [RIAxy | _ ||- e ≅ nfL : _]).
+  1: symmetry; eapply redTmEqFwd; tea; now eapply lrefl.
+  assert (RnfLR : [RIAxy | _ ||- nfL ≅ nfR : _])
+  by (eapply redTmEqFwdBoth; cycle 1; tea).
+  assert (Ryy : [RA | _ ||- y ≅ y : _]) by now eapply lrefl.
+  pose proof (RAA := reflLRTyEq RA).
+  pose proof (RPeq _ _ _ _ _ _ RAA Rxx' Ryy _ RenfL).
+  escape.
+  assert [Γ |- tId A x y ≅ tId A' x' y'] by gen_typing.
+  eapply redSubstTmEq; cycle 1; tea.
+  1,2: eapply redtm_idElim; tea.
+  1: gen_typing.
+  1-3: now eapply ty_conv.
+  1: eapply redtm_conv; tea; gen_typing.
+  eapply LRTmEqConv. 1: now eapply LRTyEqSym.
+  now unshelve eapply idElimPropCongRed.
 Qed.
 
 End IdRed.
