theories/LogicalRelation/Universe.v
@@ -13,15 +13,15 @@ Section UniverseReducibility.
     intros ?%escape; econstructor; [easy| gen_typing|eapply redtywf_refl; gen_typing].
   Qed.
 
-  Lemma UnivEq'@{i j k l} {Γ A l} (rU : [ LogRel@{i j k l} l | Γ ||- U ]) (rA : [ LogRel@{i j k l} l | Γ ||- A : U | rU])
+  Lemma UnivEq'@{i j k l} {Γ A B l} (rU : [ LogRel@{i j k l} l | Γ ||- U ]) (rA : [ LogRel@{i j k l} l | Γ ||- A ≅ B : U | rU])
     : [ LogRel@{i j k l} zero | Γ ||- A].
   Proof.
-    assert [ LogRel@{i j k l} one | Γ ||- A : U | LRU_@{i j k l} (redUOne rU)]
-             as [ _ _ _ _ hA ] by irrelevance.
+    assert [ LogRel@{i j k l} one | Γ ||- A ≅ B : U | LRU_@{i j k l} (redUOne rU)]
+             as [ ? ?? hA ] by irrelevance.
     exact (LRCumulative hA).
   Qed.
 
-  Lemma UnivEq@{i j k l} {Γ A l} l' (rU : [ LogRel@{i j k l} l | Γ ||- U]) (rA : [ LogRel@{i j k l} l | Γ ||- A : U | rU])
+  Lemma UnivEq@{i j k l} {Γ A B l} l' (rU : [ LogRel@{i j k l} l | Γ ||- U]) (rA : [ LogRel@{i j k l} l | Γ ||- A ≅ B : U | rU])
     : [ LogRel@{i j k l} l' | Γ ||- A].
   Proof.
     destruct l'.
@@ -37,31 +37,5 @@ Section UniverseReducibility.
     assert [ LogRel@{i j k l} one | Γ ||- A ≅ B : U | LRU_@{i j k l} (redUOne rU) ] as [ _ _ _ hA _ hAB ] by irrelevance.
     eapply LRTyEqIrrelevantCum. exact hAB.
   Qed.
-
-
-  (* The lemmas below does not seem to be
-     at the right levels for fundamental lemma ! *)
-
-  Set Printing Universes.
-  Lemma univTmTy'@{h i j k l} {Γ l UU A} (h : [Γ ||-U<l> UU ]) :
-    [LogRel@{i j k l} l | Γ ||- A : UU | LRU_ h] -> [LogRel@{h i j k} (URedTy.level h) | Γ ||- A].
-  Proof.  intros []; now eapply RedTyRecFwd. Qed.
-
-  Lemma univTmTy@{h i j k l} {Γ l A} (RU : [Γ ||-<l> U]) :
-    [LogRel@{i j k l} l | Γ ||- A : U | RU] -> [LogRel@{h i j k} (URedTy.level (invLRU RU)) | Γ ||- A].
-  Proof.
-    intros h; apply univTmTy'.
-    irrelevance.
-  Qed.
-
-  Lemma univEqTmEqTy'@{h i j k l} {Γ l l' UU A B} (h : [Γ ||-U<l> UU]) (RA : [Γ ||-<l'> A]) :
-    [LogRel@{i j k l} l | Γ ||- A ≅ B : UU | LRU_ h] ->
-    [LogRel@{h i j k} l' | Γ ||- A ≅ B | RA].
-  Proof. intros [????? RA']. apply TyEqRecFwd in RA'. irrelevance. Qed.
-
-  Lemma univEqTmEqTy@{h i j k l} {Γ l l' A B} (RU : [Γ ||-<l> U]) (RA : [Γ ||-<l'> A]) :
-    [LogRel@{i j k l} l | Γ ||- A ≅ B : U | RU] ->
-    [LogRel@{h i j k} l' | Γ ||- A ≅ B | RA].
-  Proof. intros h; eapply (univEqTmEqTy' (invLRU RU)); irrelevance. Qed.
 
 End UniverseReducibility.
